theories/Logic/Leaf.v
@@ -1,0 +1,86 @@
+(** * Leaves of an CTree *)
+
+From CTree Require Import
+     CTree
+     Equ.
+
+From Coq Require Import Morphisms Basics Program.Equality.
+Import CTree.
+Import CTreeNotations EquNotations.
+
+(** ** Leaves of ctree *)
+
+(** The [Leaf a t] predicate expresses that [t] has a [Ret] leaf with
+    value [a].
+
+    We provide the elementary structural lemmas to work with this
+    predicate, and one main useful result relying on [Leaf]: the
+    up-to bind closure [eqit_bind_clo] can be refined such that
+    continuations need only be related over the leaves of the
+    first operand of [bind].
+    *)
+
+Inductive Leaf {E C} {A: Type} (a: A) : ctree E C A -> Prop :=
+ | LeafRet: forall t,
+   observe t = RetF a ->
+   Leaf a t
+ | LeafTau: forall {X} (c: C X) b t k x,
+   observe t = BrF b c k ->
+   Leaf a (k x) ->
+   Leaf a t
+ | LeafVis: forall {X} (e: E X) t k x,
+   observe t = VisF e k ->
+   Leaf a (k x) ->
+   Leaf a t.
+#[global] Hint Constructors Leaf : ctree.
+
+Notation "a ∈ t" := (Leaf a t) (at level 70).
+
+(** Smart constructors *)
+Lemma Leaf_Ret : forall E C R a,
+  a ∈ (Ret a : ctree E C R).
+Proof.
+  intros; econstructor; reflexivity.
+Qed.
+
+Lemma Leaf_Br : forall E X Y C b (c: C X) (k: _ -> ctree E C Y) a x,
+  a ∈ k x ->
+  a ∈ Br b c k.
+Proof.
+  intros; econstructor; [reflexivity | eauto].
+Qed.
+
+Lemma Leaf_Vis : forall E C X Y (e : E X) (k : _ -> ctree E C Y) b x,
+  b ∈ (k x) ->
+  b ∈ (Vis e k).
+Proof.
+  intros * IN; econstructor 3; [reflexivity | eauto].
+Qed.
+
+(** Inversion lemmas *)
+Lemma Leaf_Ret_inv : forall E C R (a b : R),
+  Leaf (E := E) (C := C) b (Ret a) ->
+  b = a.
+Proof.
+  intros * IN; inv IN; cbn in *; try congruence.
+Qed.
+
+Lemma Leaf_Tau_inv : forall E C X Y (c: C X) (k: _ -> ctree E C Y) b a,
+  a ∈ Br b c k ->
+  exists x, a ∈ k x.
+Proof.
+  intros * IN *; inv IN; cbn in *; try congruence.
+  revert x H0.
+  refine (match H in _ = u return match u with BrF b c0 k0 =>  _ | _ => False end with eq_refl => _ end).
+  eauto.
+Qed.
+
+Lemma Leaf_Vis_inv : forall E C X Y (e : E X) (k : _ -> ctree E C Y) b,
+  b ∈ Vis e k ->
+  exists x, b ∈ k x.
+Proof.
+  intros * IN *; inv IN; cbn in *; try congruence.
+  revert x H0.
+  refine (match H in _ = u return match u with VisF c0 k0 =>  _ | _ => False end with eq_refl => _ end).
+  eauto.
+Qed.
